\documentclass{article}

\usepackage{amsthm,amsmath,amssymb}

\begin{document}
		
	\section*{3.1}
		$$
		\begin{gathered}
		p_{Y}(1)=P(X \leq \frac{1}{3})=\frac{1}{3} \\
		p_{Y}(2)=1-p_{Y}(1)=\frac{2}{3} \\
		E[Y]=\frac{1}{3} \times 1+\frac{2}{3} \times 2=\frac{5}{3} \\
		E[Y]=\int_{0}^{1} g(x) f_{X}(x) d x=\int_{0}^{\frac{1}{3}} d x+\int_{\frac{1}{3}}^{1} 2 d x=\frac{5}{3}
		\end{gathered}
		$$
	\section*{3.5}
		$$
		\begin{gathered}
		F_{X}(x)=1-P(X>x)=1-\frac{A_{x}}{A}=1-\frac{b(h-x)^{2} /(2 h)}{b h / 2}=1-\left(\frac{h-x}{h}\right)^{2}, \\
		f_{X}(x)=\frac{d F_{X}}{d x}(x)= \begin{cases}\frac{2(h-x)}{h^{2}}, & \text { if } 0 \leq x \leq h, \\
		0, & \text { otherwise. }\end{cases}
		\end{gathered}
		$$

	
	\section*{3.13}
	
		$$
		\begin{gathered}
		P(Y \leq 59)=P(X \leq 15)=P\left(Z \leq \frac{15-E[X]}{\sigma_{X}}\right)=P(Z \leq 0.5)=\Phi(0.5) \\
		\Phi(0.5)=0.6915 \\
		P(Y \leq 59)=0.6915
		\end{gathered}
		$$

	\section*{2.21}
		\begin{equation}
		f_{X \mid Y}(x \mid y)=1 / y, \text { for } 0 \leq x \leq y
		\end{equation}

		$$
		\begin{gathered}
		f_{X, Y}(x, y)=f_{Y}(y) f_{X \mid Y}(x \mid y)= \begin{cases}\frac{1}{l} \times \frac{1}{y}, & 0 \leq x \leq y \leq l \\
		0, & \text { otherwise. }\end{cases} \\
		f_{X}(x)=\int f_{X, Y}(x, y) d y=\int_{x}^{l} \frac{1}{l y} d y=\frac{1}{l} \ln (l / x), \quad 0 \leq x \leq l . \\
		E[X]=\int_{0}^{l} x f_{X}(x) d x=\int_{0}^{l} \frac{x}{l} \ln (l / x) d x=\frac{l}{4}
		\end{gathered}
		$$
		$$
		\begin{gathered}
		E[Y]=l / 2 \\
		E[X / Y]=1 / 2 \\
		E[X]=E[Y] E\left[\frac{X}{Y}\right]=\frac{l}{2} \cdot \frac{1}{2}=\frac{l}{4}
		\end{gathered}
		$$

			
		
	\section*{2.25}
	
		$A$ : $X^{2}+Y^{2} \geq c^{2}$.
		$$
		\begin{aligned}
		P(A) &=\frac{1}{2 \pi \sigma^{2}} \int_{0}^{2 \pi} \int_{a}^{\infty} r e^{-r^{2} / 2 \sigma^{2}} d r d \theta \\
		&=\frac{1}{\sigma^{2}} \int_{a}^{\infty} r e^{-r^{2} / 2 \sigma^{2}} d r \\
		&=e^{-a^{2} / 2 \sigma^{2}}
		\end{aligned}
		$$
		$$
		f_{X, Y \mid A}(x, y)=\frac{f_{X, Y}(x, y)}{P(A)}=\frac{1}{2 \pi \sigma^{2}} e^{-\frac{1}{2 \sigma^{2}}\left(x^{2}+y^{2}-c^{2}\right)}
		$$



\end{document}